refactoring

theories/Means.ec
@@ -160,6 +160,7 @@ theory Hybrid.
   type input.
   type output.
   type leaks.
+  op in0 : input.
 
   module type Enc = { 
     fun init () : unit { * }
@@ -175,12 +176,8 @@ theory Hybrid.
   module type LR = { 
     fun lr(m0 m1:input) : output
   }.
-
-  module type Mk_LR(E:AEnc) = {
-    fun lr(m0 m1:input) : output
-  }.
-    
-(*  module L(E:Enc) = {
+   
+  module L(E:Enc) = {
     fun lr(m0 m1:input) : output = {
       var r : output;
       r = E.enc(m0);
@@ -195,60 +192,218 @@ theory Hybrid.
       return r;
     }
   }. 
-*)
 
-  module type Adv(E:AEnc, LR:LR) = {
+  module type E0Adv(E:AEnc, E0:AEnc) = {
     fun run () : bool
   }.
 
   import Int.
 
-  module N (E:Enc, LR:LR, A:Adv) = {
-    var c:int
+  module C = { 
+    var c : int
+    fun init () : unit = {
+      c = 0;
+    }
+    fun incr () : unit = {
+      c = c + 1;
+    }
+  }.
 
-    module LRc = {
-      fun lr(m0 m1:input) : output = {
+  module G_E (A:E0Adv, E:Enc) = {
+    module Em = {
+      fun leaks () : leaks = { (* TODO: be able to write fun leaks = E.leaks *)
+        var r : leaks;
+        r = E.leaks();
+        return r;
+      }
+
+      fun enc(m:input) : output = {
         var r : output;
-        c = c + 1;
-        r = LR.lr(m0, m1);
+        r = E.enc(m);
+        C.incr();
         return r;
       }
     }
-
-    module A = A(E,LRc)
+      
+    module A = A(E,Em)
 
     fun main () : bool = {
       var b' : bool;
-      c = 0;        
       E.init();
+      C.init();
       b' = A.run();
       return b';
     }
   }.
 
-  op q : int.
+  module G_E0(A:E0Adv, E:Enc) = {
+    module E0 = {
+      
+      fun leaks () : leaks = { (* TODO: be able to write fun leaks = E.leaks *)
+        var r : leaks;
+        r = E.leaks();
+        return r;
+      }
 
-  clone import Mean as M with
-    type input <- int,
-    type output <- bool,
-    op d <- [0..q-1].
+      fun enc(m:input) : output = {
+        var r : output;
+        r = E.enc(in0);
+        C.incr();
+        return r;
+      }
+    }
+    module A = A(E,E0)
 
-  module LRB (L: LR, R: LR, LR0:LR) = {
+    fun main () : bool = {
+      var b' : bool;
+      E.init();
+      C.init();
+      b' = A.run();
+      return b';
+    }
+  }.
+
+  module type LRAdv(E:AEnc, LR:LR) = {
+    fun run () : bool
+  }.
+
+  module GL(A:LRAdv, E:Enc) = {
+    module L = { 
+      fun lr(m0 m1:input) : output = {
+        var r : output;
+        r = E.enc(m0);
+        C.incr();
+        return r;
+      }
+    }
+    module A = A(E,L)
+    fun main () : bool = {
+      var b' : bool;
+      E.init();
+      C.init();
+      b' = A.run();
+      return b';
+    }
+  }.
+
+  module GR(A:LRAdv, E:Enc) = {
+    module R = {
+      fun lr(m0 m1:input) : output = {
+        var r : output;
+        r = E.enc(m1);
+        C.incr();
+        return r;
+      }
+    }
+    module A = A(E,R)
+    fun main () : bool = {
+      var b' : bool;
+      E.init();
+      C.init();
+      b' = A.run();
+      return b';
+    }
+  }.
+
+  module BLR(A:E0Adv, E:AEnc, LR:LR) = {
+    module E0 = {
+      fun leaks () : leaks = { (* TODO: be able to write fun leaks = E.leaks *)
+        var r : leaks;
+        r = E.leaks();
+        return r;
+      }
+
+      fun enc(m:input) : output = {
+        var r : output;
+        r = LR.lr(m, in0);
+        return r;
+      }
+    }
+    module A = A(E,E0)
+    fun run () : bool = {
+      var b' : bool;
+      b' = A.run();
+      return b';
+    }
+  }.
+
+  equiv Cinit : C.init ~ C.init : true ==> ={C.c}.
+  proof strict.
+   by fun;wp.
+  qed.
+
+  equiv Cincr : C.incr ~ C.incr : ={C.c} ==> ={C.c}.
+  proof strict.
+    by fun;wp.
+  qed.
+
+ 
+  section. (* E0_LR. *)
+    declare module E : Enc{C}.
+    declare module A : E0Adv{E,C}.
+
+    equiv GE_GL : G_E(A,E).main ~ GL(BLR(A),E).main : ={glob A} ==> ={res,glob A,C.c}.
+    proof strict.
+      fun;inline{2} GL(BLR(A), E).A.run;wp.
+      call (_: ={glob E, C.c}).
+        by fun;call (_: true).
+        fun;inline{2} GL(BLR(A), E).L.lr;wp.
+        by call Cincr; call(_: true);wp.
+        by fun (={C.c}).
+        by fun (={C.c}).
+      by call Cinit;call (_ : true).
+    qed.
+
+    equiv GE0_GR : G_E0(A,E).main ~ GR(BLR(A),E).main : ={glob A} ==> ={res,glob A}.
+    proof strict.
+      fun;inline{2} GR(BLR(A), E).A.run;wp.
+      call (_: ={glob E,C.c}).
+        by fun;call (_: true).
+        fun; inline{2} GR(BLR(A), E).R.lr;wp.
+        by call Cincr; call(_: true);wp.
+        by fun (={C.c}).
+        by fun (={C.c}).
+      by call Cinit;call (_ : true).
+    qed.
+
+    lemma E0_LR &m (p:glob A -> bool): 
+      Pr[G_E(A,E).main() @ &m : res /\ p (glob A) ] - 
+      Pr[G_E0(A,E).main() @ &m : res /\ p (glob A) ] =
+      Pr[GL(BLR(A),E).main() @ &m : res /\ p (glob A)] -
+      Pr[GR(BLR(A),E).main() @ &m : res /\ p (glob A)].
+    proof.
+      congr;first by equiv_deno GE0_GR.
+      by equiv_deno GE_GL.
+    qed.
+
+  end section.
+
+   module LRB (E:AEnc,LR:LR) = {
     var l, l0 : int  
     fun lr(m0 m1:input):output = {
       var r : output;
-      if (l0 < l) r = L.lr(m0,m1);
+      if (l0 < l) r = E.enc(m0);
       else { 
-        if (l0 = l) r = LR0.lr(m0,m1);
-        else r = R.lr(m0,m1);
+        if (l0 = l) r = LR.lr(m0,m1);
+        else r = E.enc(m1);
       }
       l = l + 1;
       return r;
     }
+
+      fun enc(m:input) : output = {
+        var r : output;
+        r = E.enc(in0);
+        C.incr();
+        return r;
+      }
+    
   }.
- 
-  module B(A:Adv, L:LR, R:LR, E:AEnc, LR0:LR) = {
-    module LR = LRB(L,R,LR0)
+  
+  op q : int.
+  
+  module B(A:LRAdv, E:AEnc, LR0:LR) = {
+    module LR = LRB(E,LR0)
     module A = A(E,LR)
     fun run():bool = {
       var b':bool;
@@ -259,267 +414,234 @@ theory Hybrid.
     }
   }.
 
+  clone import Mean as M with
+    type input <- int,
+    type output <- bool,
+    op d <- [0..q-1].
+
   section.
 
-  declare module E    : Enc   {N,LRB}.
-  declare module ML   : Mk_LR {N,LRB,E}.
-  declare module MR   : Mk_LR {N,LRB,E,ML}.  
-  declare module A    : Adv   {N,LRB,E,ML,MR}.
-  
-  local module L   = ML(E).
-  local module R   = MR(E).
-  local module LRBL = LRB(L,R,L).
-  local module LRBR = LRB(L,R,R).
+    declare module E    : Enc   {C,LRB}.
+    declare module A    : LRAdv   {C,LRB,E}.
 
-  local module BA  = B(A, L, R).
-  local module NLB = N(E,L,BA).
-  local module NRB = N(E,R,BA).  
+    local module W (LR0:LR) = {
+      module LR = LRB(E,LR0)
+      module A = A(E,LR)
+      fun work(x:int) : bool = {
+        var b':bool;
+        LRB.l = 0; LRB.l0 = x;
+        E.init();
+        b' = A.run();
+        return b' /\ LRB.l <= q;
+      }
+    }.
 
+    local equiv Einit : E.init ~ E.init : true ==> ={glob E}.
+    proof strict. by fun true. qed.
 
-  local module W (LR0:LR) = {
-    module LR = LRB(L,R,LR0)
-    module A = A(E,LR)
-    fun work(x:int) : bool = {
-      var b':bool;
-      LRB.l = 0; LRB.l0 = x;
-      E.init();
-      b' = A.run();
-      return b' && LRB.l <= q;
-    }
-  }.
+    local equiv Eleaks : E.leaks ~ E.leaks : ={glob E} ==> ={res,glob E}.
+    proof strict. by fun true. qed.
 
-  local equiv Einit : E.init ~ E.init : true ==> ={glob E}.
-  proof strict.
-    by fun true.
-  qed.
+    local equiv Eenc : E.enc ~ E.enc : ={m,glob E} ==> ={res,glob E}.
+    proof strict. by fun true. qed.
 
-  local equiv Eleaks : E.leaks ~ E.leaks : ={glob E} ==> ={res,glob E}.
-  proof strict.
-    by fun true.   
-  qed.
+    local lemma GLB_WL &m :
+      Pr[GL(B(A),E).main() @ &m : res /\ C.c <= 1] = 
+      Pr[Rand(W(L(E))).randAndWork() @ &m : snd res].
+    proof strict.
+      equiv_deno (_ : ={glob A} ==> res{1} = snd res{2} /\ C.c{1} <= 1) => //.
+      fun; inline{1} GL(B(A), E).A.run;inline{2} W(L(E)).work;wp.
+      call (_: ={glob E, glob LRB} /\ C.c{1} = (LRB.l0{1} < LRB.l{1}) ? 1 : 0).
+        fun;wp.
+        if => //;first by call Eenc;skip;progress => //; smt.
+        if => //.
+          inline{1} GL(B(A), E).L.lr C.incr;inline{2} L(E).lr.
+          by wp;call Eenc;wp;skip;progress => //;smt.
+        by call Eenc;skip;progress => //; smt.
+        by conseq * Eleaks.
+        by conseq * Eenc.
+      swap{1} 1 3;inline{1} C.init.
+      by call Einit;wp;rnd;wp;skip;progress => //;smt.
+    qed.
 
-  local equiv Eenc : E.enc ~ E.enc : ={m,glob E} ==> ={res,glob E}.
-  proof strict.
-    by fun true.   
-  qed.
+    local lemma GRB_WR &m :
+      Pr[GR(B(A),E).main() @ &m : res /\ C.c <= 1] = 
+      Pr[Rand(W(R(E))).randAndWork() @ &m : snd res].
+    proof strict.
+      equiv_deno (_ : ={glob A} ==> 
+                      res{1} = snd res{2} /\ C.c{1} <= 1) => //.
+      fun; inline{1} GR(B(A), E).A.run;inline{2} W(R(E)).work;wp.
+      call (_: ={glob E, glob LRB} /\ C.c{1} = (LRB.l0{1} < LRB.l{1}) ? 1 : 0).
+        fun;wp.
+        if => //;first by wp;call Eenc;skip;progress => //; smt.
+        if => //.
+          inline{1} GR(B(A), E).R.lr C.incr;inline{2} R(E).lr.
+          by wp;call Eenc;wp;skip;progress => //;smt.
+        by call Eenc;skip;progress => //; smt.
+        by conseq * Eleaks.
+        by conseq * Eenc.
+      swap{1} 1 3;inline{1} C.init.
+      by call Einit;wp;rnd;wp;skip;progress => //;smt.
+    save.
 
-  local equiv Eml : ML(E).lr ~ ML(E).lr : ={m0,m1,glob ML, glob E} ==> ={res, glob ML, glob E}.
-  proof strict.
-    fun (={glob E})=> //;[apply Eleaks | apply Eenc].
-  qed.
+    axiom losslessA (E0 <: AEnc{A}) (LR <: LR{A}):
+        islossless LR.lr =>
+        islossless E0.leaks => islossless E0.enc => islossless A(E0, LR).run.
+    axiom losslessL: islossless E.leaks.
+    axiom losslessE: islossless E.enc.
 
-  local equiv Emr : MR(E).lr ~ MR(E).lr : ={m0,m1,glob MR, glob E} ==> ={res, glob MR, glob E}.
-  proof strict.
-    fun (={glob E})=> //;[apply Eleaks | apply Eenc].
-  qed.
- 
-  local lemma NWL &m :
-    Pr[N(E,L,BA).main() @ &m : res /\ N.c <= 1] = 
-    Pr[Rand(W(L)).randAndWork() @ &m : snd res].
-  proof strict.
-    equiv_deno (_ : ={glob A, glob ML, glob MR} ==> 
-                    res{1} = snd res{2} /\ N.c{1} <= 1) => //.
-    fun. 
-    inline{1} N(E, ML(E), B(A, ML(E), MR(E))).A.run.
-    inline{2} W(ML(E)).work;wp.
-    call (_: ={glob ML, glob MR, glob E, glob LRB} /\ N.c{1} = (LRB.l0{1} < LRB.l{1}) ? 1 : 0).
-      fun;wp.
-      if => //.
-        by call Eml;skip;progress => //; smt.
-      if => //.
-        inline{1} N(E, ML(E), B(A, ML(E), MR(E))).LRc.lr;wp.
-        by call Eml;wp;skip;progress => //;smt.
-      by call Emr;skip;progress => //; smt.
-      by conseq * Eleaks.
-      by conseq * Eenc.
-    swap{1} 2 2.
-    by call Einit;wp;rnd;wp;skip;progress => //;smt.
-  qed.
+    axiom q_pos : 0 < q.
 
-  local lemma NWR &m :
-    Pr[N(E,R,BA).main() @ &m : res /\ N.c <= 1] = 
-    Pr[Rand(W(R)).randAndWork() @ &m : snd res].
-  proof strict.
-    equiv_deno (_ : ={glob A, glob ML, glob MR} ==> 
-                    res{1} = snd res{2} /\ N.c{1} <= 1) => //.
-    fun. 
-    inline{1} N(E, MR(E), B(A, ML(E), MR(E))).A.run.
-    inline{2} W(MR(E)).work;wp.
-    call (_: ={glob ML, glob MR, glob E, glob LRB} /\ N.c{1} = (LRB.l0{1} < LRB.l{1}) ? 1 : 0).
-      fun;wp.
-      if => //.
-        by call Eml;skip;progress => //; smt.
-      if => //.
-        inline{1} N(E, MR(E), B(A, ML(E), MR(E))).LRc.lr;wp.
-        by call Emr;wp;skip;progress => //;smt.
-      by call Emr;skip;progress => //; smt.
-      by conseq * Eleaks.
-      by conseq * Eenc.
-    swap{1} 2 2.
-    by call Einit;wp;rnd;wp;skip;progress => //;smt.
-  save.
-
-  axiom losslessA (E0 <: AEnc{A}) (LR <: LR{A}):
-      islossless LR.lr =>
-      islossless E0.leaks => islossless E0.enc => islossless A(E0, LR).run.
-  axiom losslessML (E0 <: AEnc{ML}):
-    islossless E0.leaks => islossless E0.enc => islossless ML(E0).lr.
-  axiom losslessMR (E0 <: AEnc{MR}):
-    islossless E0.leaks => islossless E0.enc => islossless MR(E0).lr.
-  axiom losslessL: islossless E.leaks.
-  axiom losslessE: islossless E.enc.
-
-  local lemma losslessMLE : islossless ML(E).lr.
-  proof strict.
-    apply (losslessML E);[apply losslessL | apply losslessE].
-  qed.
-
-  local lemma losslessMRE : islossless MR(E).lr.
-  proof strict.
-    apply (losslessMR E);[apply losslessL | apply losslessE].
-  qed.
-  
-  axiom q_pos : 0 < q.
-
-  local lemma WL0_NLA &m: 
-     Pr[W(L).work(0) @ &m : res] = Pr[N(E,L,A).main() @ &m : res /\ N.c <= q ].
-  proof strict.
-    equiv_deno (_ : ={glob A, glob ML, glob MR} /\ x{1}=0 ==> 
-                    res{1} = (res{2} /\ N.c{2} <= q)) => //.
-    fun.
-    call (_: q < N.c,
-             ={glob ML, glob MR, glob E} /\ LRB.l0{1} = 0 /\ LRB.l{1} = N.c{2} /\ 0 <= LRB.l{1},
-             LRB.l0{1} = 0 /\ q < LRB.l{1}).
-      by apply losslessA.
-
+    local lemma WL0_GLA &m: 
+       Pr[W(L(E)).work(0) @ &m : res] = Pr[GL(A,E).main() @ &m : res /\ C.c <= q ].
+    proof strict.
+      equiv_deno (_ : ={glob A} /\ x{1}=0 ==> 
+                      res{1} = (res{2} /\ C.c{2} <= q)) => //.
       fun.
-      if{1}.
-        by wp;call Eml;wp;skip;progress => //;smt.
-      rcondt{1} 1.
-        by intros &m0;skip;smt.
-      by wp;call Eml;wp;skip;progress => //;smt.
-      intros &m2 _;fun.
-      rcondt 1; first by skip;smt.
-      by wp;call losslessMLE;skip;smt.
-      intros &m1;fun.
-      by call losslessMLE;wp;skip;smt.
-      
-      by conseq * Eleaks.
-      intros &m2 _;conseq * losslessL.
-      intros &m1; conseq * losslessL.
+      call (_: q < C.c,
+               ={glob E} /\ LRB.l0{1} = 0 /\ LRB.l{1} = C.c{2} /\ 0 <= LRB.l{1},
+               LRB.l0{1} = 0 /\ q < LRB.l{1}).
+        by apply losslessA.
 
-      by conseq * Eenc.
-      intros &m2 _;conseq * losslessE.
-      intros &m1; conseq * losslessE.
-    
-    by call Einit;wp;skip;progress => //;smt.
-  qed.
+        fun;inline{2} C.incr;wp.
+        if{1};first by call Eenc;skip;progress => //;smt.
+        rcondt{1} 1; first by intros &m0;skip;smt.
+        by inline{1} L(E).lr;wp;call Eenc;wp;skip;progress => //;smt.
+        intros &m2 _;fun.
+        rcondt 1; first by skip;smt.
+        by wp;call losslessE;skip;smt.
+        by intros &m1;fun;inline C.incr;wp;call losslessE;wp;skip;smt.
 
-  local lemma WRq_NRA &m: 
-     Pr[W(R).work((q-1)) @ &m : res] = Pr[N(E,R,A).main() @ &m : res /\ N.c <= q ].
-  proof strict.
-    equiv_deno (_ : ={glob A, glob ML, glob MR} /\ x{1}=q-1 ==> 
-                    res{1} = (res{2} /\ N.c{2} <= q)) => //.
-    fun.
-    call (_: q < N.c,
-             ={glob ML, glob MR, glob E} /\ LRB.l0{1} = q-1 /\ LRB.l{1} = N.c{2} /\ 0 <= LRB.l{1},
-             LRB.l0{1} = q-1 /\ q < LRB.l{1}).
-      by apply losslessA.
+        by conseq * Eleaks.
+        intros &m2 _;conseq * losslessL.
+        intros &m1; conseq * losslessL.
 
+        by conseq * Eenc.
+        intros &m2 _;conseq * losslessE.
+        intros &m1; conseq * losslessE.
+
+      by inline{2} C.init;wp;call Einit;wp;skip;progress => //;smt.
+    qed.
+
+    local lemma WRq_GRA &m: 
+       Pr[W(R(E)).work((q-1)) @ &m : res] = Pr[GR(A,E).main() @ &m : res /\ C.c <= q ].
+    proof strict.
+      equiv_deno (_ : ={glob A} /\ x{1}=q-1 ==> 
+                      res{1} = (res{2} /\ C.c{2} <= q)) => //.
       fun.
-      if{1}.
-        by wp;call{1} losslessMLE;call{2} losslessMRE;wp;skip; smt.
-      if{1}.
-        by wp;call Emr;wp;skip;progress => //;smt.
-      by wp;call Emr;wp;skip;progress => //;smt.
-      intros &m2 _;fun.
-      rcondt 1; first by skip;smt.
-      by wp;call losslessMLE;skip; smt.
-      by intros &m1;fun;call losslessMRE;wp;skip;smt.
-      
-      by conseq * Eleaks.
-      intros &m2 _;conseq * losslessL.
-      intros &m1; conseq * losslessL.
+      call (_: q < C.c,
+               ={glob E} /\ LRB.l0{1} = q-1 /\ LRB.l{1} = C.c{2} /\ 0 <= LRB.l{1},
+               LRB.l0{1} = q-1 /\ q < LRB.l{1}).
+        by apply losslessA.
 
-      by conseq * Eenc.
-      intros &m2 _;conseq * losslessE.
-      intros &m1; conseq * losslessE.
-    
-    by call Einit;wp;skip;progress => //;smt.
-  qed.
+        fun;inline{2} C.incr;wp.
+        if{1};first by call{1} losslessE;call{2} losslessE;skip; smt.
+        inline{1} R(E).lr;if{1};first by wp;call Eenc;wp;skip;progress => //;smt.
+        by call Eenc;skip;progress => //;smt.
+        intros &m2 _;fun.
+        rcondt 1; first by skip;smt.
+        by wp;call losslessE;skip; smt.
+        by intros &m1;fun;inline C.incr;wp;call losslessE;wp;skip;smt.
 
-  local lemma WLR_shift &m v: 1 <= v <= q-1 => 
-       Pr[W(L).work(v) @ &m: res] = Pr[W(R).work((v-1)) @ &m : res].
-  proof strict.
-    intros Hv;equiv_deno (_: ={glob A, glob ML, glob MR} /\ x{1} = v /\ x{2} = v-1 ==> ={res}) => //.
-    fun.
-    call (_: ={glob ML, glob MR, glob E, LRB.l} /\ LRB.l0{1} = v /\ LRB.l0{2} = v-1).
+        by conseq * Eleaks.
+        intros &m2 _;conseq * losslessL.
+        intros &m1; conseq * losslessL.
+
+        by conseq * Eenc.
+        intros &m2 _;conseq * losslessE.
+        intros &m1; conseq * losslessE.
+
+      by inline{2} C.init;wp;call Einit;wp;skip;progress => //;smt.
+    qed.
+
+    local lemma WLR_shift &m v: 1 <= v <= q-1 => 
+         Pr[W(L(E)).work(v) @ &m: res] = Pr[W(R(E)).work((v-1)) @ &m : res].
+    proof strict.
+      intros Hv;equiv_deno (_: ={glob A} /\ x{1} = v /\ x{2} = v-1 ==> ={res}) => //.
       fun.
-      if{1}.        
-        rcondt{2} 1;first by intros &m0;skip;smt.
-        by wp;call Eml.
-      if{1}.
-        rcondt{2} 1;first by intros &m0;skip;smt.
-        by wp;call Eml.
-      rcondf{2} 1;first by intros &m0;skip;smt.
-      by if{2};wp;call Emr.
-      by conseq * Eleaks.
-      by conseq * Eenc.
-    by call Einit;wp.
-  qed.
+      call (_: ={glob E, LRB.l} /\ LRB.l0{1} = v /\ LRB.l0{2} = v-1).
+        fun.
+        if{1}; first by rcondt{2} 1;[intros &m0;skip;smt | wp;call Eenc].
+        if{1};first by rcondt{2} 1;[intros &m0;skip;smt | inline{1} L(E).lr;wp;call Eenc;wp].
+        rcondf{2} 1;first by intros &m0;skip;smt.
+        by inline{2} R(E).lr;if{2};wp;call Eenc;wp.
+        by conseq * Eleaks.
+        by conseq * Eenc.
+      by call Einit;wp.
+    qed.
 
-  (* TODO : move this *)
-  lemma Mrplus_inter_shift (i j k:int) f: 
-      Mrplus.sum f (Interval.interval i j) = 
-      Mrplus.sum (lambda l, f (l + k)) (Interval.interval (i-k) (j-k)).
-  proof strict.
-    rewrite (Mrplus.sum_chind f (lambda l, l - k) (lambda l, l + k)) /=;first smt.
-    congr => //.   
-    apply FSet.set_ext => x.
-    rewrite img_def Interval.mem_interval;split.
-      intros [y];rewrite Interval.mem_interval;smt.
-    intros Hx;exists (x+k);rewrite Interval.mem_interval;smt.
-  qed.
-
-  lemma Hybrid &m : 
-     Pr[N(E,ML(E),B(A,ML(E),MR(E))).main() @ &m : res /\ N.c <= 1] - 
-        Pr[N(E,MR(E),B(A,ML(E),MR(E))).main() @ &m : res /\ N.c <= 1] = 
-     1%r/q%r * (
-       Pr[N(E,ML(E),A).main() @ &m : res /\ N.c <= q] - 
-         Pr[N(E,MR(E),A).main() @ &m : res /\ N.c <= q]).
-  proof strict.
-    rewrite (NWL &m) (NWR &m) -(WL0_NLA &m) -(WRq_NRA &m).
-    cut Hint : Finite.(==) (create (support [0..q - 1])) (Interval.interval 0 (q - 1)).
-      by intros x;rewrite mem_create Interval.mem_interval /support Dinter.supp_def.
-    cut Hfin: Finite.finite (create (support [0..q - 1])).
-      by exists (Interval.interval 0 (q-1)).
-    cut Huni : forall (x : int), in_supp x [0..q - 1] => mu_x [0..q - 1] x = 1%r / q%r.
-      by intros x Hx;rewrite Dinter.mu_x_def_in //;smt.
-    cut := M.Mean_uni (W(L)) &m (lambda j g r, r) (1%r/q%r) _ _ => // /= ->.
-    cut := M.Mean_uni (W(R)) &m (lambda j g r, r) (1%r/q%r) _ _ => // /= ->.
-    cut -> : Finite.toFSet (create (support [0..q - 1])) = Interval.interval 0 (q-1).
+    (* TODO : move this *)
+    lemma Mrplus_inter_shift (i j k:int) f: 
+        Mrplus.sum f (Interval.interval i j) = 
+        Mrplus.sum (lambda l, f (l + k)) (Interval.interval (i-k) (j-k)).
+    proof strict.
+      rewrite (Mrplus.sum_chind f (lambda l, l - k) (lambda l, l + k)) /=;first smt.
+      congr => //.   
       apply FSet.set_ext => x.
-      by rewrite Interval.mem_interval Finite.mem_toFSet // mem_create /support Dinter.supp_def.
-    rewrite {1}Interval.interval_addl;first by smt.
-    rewrite (Interval.interval_pos 0 (q-1));first by smt.
-    rewrite Mrplus.sum_add /=.
-      by rewrite Interval.mem_interval.
-    rewrite Mrplus.sum_add /=.
-      by rewrite Interval.mem_interval;smt.
-    cut Hq : q%r <> Real.zero by smt.
-    fieldeq => //.
-    rewrite -(Mrplus.sum_comp (( * ) (-1)%r)) //;first intros x y;ringeq.
-    rewrite (Mrplus_inter_shift 0 (q - 1 - 1) (-1)) /=.
-    cut -> : q - 1 - 1 - -1 = q - 1; first by smt.
-    rewrite Mrplus.sum_add2.
-    rewrite (Mrplus.NatMul.sum_const 0%r) /Mrplus.NatMul.( * ) /=;last ringeq.
-    intros x; rewrite Interval.mem_interval => Hx;rewrite (WLR_shift &m x) //.
-      (* cut -> : x + -1 = x - 1     BUG *) 
-    by smt.
-  qed.
+      rewrite img_def Interval.mem_interval;split.
+        intros [y];rewrite Interval.mem_interval;smt.
+      intros Hx;exists (x+k);rewrite Interval.mem_interval;smt.
+    qed.
+
+    lemma Hybrid &m : 
+       Pr[GL(B(A),E).main() @ &m : res /\ C.c <= 1] - 
+         Pr[GR(B(A),E).main() @ &m : res /\ C.c <= 1] = 
+       1%r/q%r * (
+         Pr[GL(A,E).main() @ &m : res /\ C.c <= q] - 
+           Pr[GR(A,E).main() @ &m : res /\ C.c <= q]).
+    proof strict.
+      rewrite (GLB_WL &m) (GRB_WR &m) -(WL0_GLA &m) -(WRq_GRA &m).
+      cut Hint : Finite.(==) (create (support [0..q - 1])) (Interval.interval 0 (q - 1)).
+        by intros x;rewrite mem_create Interval.mem_interval /support Dinter.supp_def.
+      cut Hfin: Finite.finite (create (support [0..q - 1])).
+        by exists (Interval.interval 0 (q-1)).
+      cut Huni : forall (x : int), in_supp x [0..q - 1] => mu_x [0..q - 1] x = 1%r / q%r.
+        by intros x Hx;rewrite Dinter.mu_x_def_in //;smt.
+      cut := M.Mean_uni (W(L(E))) &m (lambda j g r, r) (1%r/q%r) _ _ => // /= ->.
+      cut := M.Mean_uni (W(R(E))) &m (lambda j g r, r) (1%r/q%r) _ _ => // /= ->.
+      cut -> : Finite.toFSet (create (support [0..q - 1])) = Interval.interval 0 (q-1).
+        apply FSet.set_ext => x.
+        by rewrite Interval.mem_interval Finite.mem_toFSet // 
+             mem_create /support Dinter.supp_def.
+      rewrite {1}Interval.interval_addl;first by smt.
+      rewrite (Interval.interval_pos 0 (q-1));first by smt.
+      rewrite Mrplus.sum_add /=.
+        by rewrite Interval.mem_interval.
+      rewrite Mrplus.sum_add /=.
+        by rewrite Interval.mem_interval;smt.
+      cut Hq : q%r <> Real.zero by smt.
+      fieldeq => //.
+      rewrite -(Mrplus.sum_comp (( * ) (-1)%r)) //;first intros x y;ringeq.
+      rewrite (Mrplus_inter_shift 0 (q - 1 - 1) (-1)) /=.
+      cut -> : q - 1 - 1 - -1 = q - 1; first by smt.
+      rewrite Mrplus.sum_add2.
+      rewrite (Mrplus.NatMul.sum_const 0%r) /Mrplus.NatMul.( * ) /=;last ringeq.
+      intros x; rewrite Interval.mem_interval => Hx;rewrite (WLR_shift &m x) //.
+        (* cut -> : x + -1 = x - 1     BUG *) 
+      by smt.
+    qed.
 
   end section.
+(*
+print axiom Hybrid.
 
-end Hybrid.
+  lemma Hybrid0 (E <: Enc{C, LRB}) (A <: E0Adv{C, LRB, E}) : 
+    (forall (E0 <: AEnc{A}) (LR <: LR{A}),
+       islossless LR.lr =>
+       islossless E0.leaks => islossless E0.enc => islossless A(E0, LR).run) => *)
+    islossless E.leaks =>
+    islossless E.enc =>
+    0 < q =>
+    forall &m,
+      Pr[G_E(B(BLR(A), E).main() @ &m : res /\ C.c <= 1] -
+      Pr[G_E0(B(A), E).main() @ &m : res /\ C.c <= 1] =
+      1%r / q%r *
+      (Pr[GL(A, E).main() @ &m : res /\ C.c <= q] -
+       Pr[GR(A, E).main() @ &m : res /\ C.c <= q]).
 
-
+lemma E0_LR:  &m (p:glob A -> bool): 
+      Pr[G_E(A,E).main() @ &m : res /\ p (glob A) ] - 
+      Pr[G_E0(A,E).main() @ &m : res /\ p (glob A) ] =
+      Pr[GL(BLR(A),E).main() @ &m : res /\ p (glob A)] -
+      Pr[GR(BLR(A),E).main() @ &m : res /\ p (glob A)].
+*)
